ModSim + PCM w/o stuttering index

src/ModSim.v
@@ -4,13 +4,16 @@ Require Export Coq.Strings.String.
 Require Import Coq.Classes.RelationClasses.
 
 From Fairness Require Export ITreeLib FairBeh Mod.
-From Fairness Require Import pind8.
+From Fairness Require Import pind.
+From Fairness Require Import PCM.
 
 Set Implicit Arguments.
 
 
 
 Section PRIMIVIESIM.
+  Context `{M: URA.t}.
+
   Variable state_src: Type.
   Variable state_tgt: Type.
 
@@ -25,194 +28,183 @@ Section PRIMIVIESIM.
   Let srcE := ((@eventE _ident_src +' cE) +' sE state_src).
   Let tgtE := ((@eventE _ident_tgt +' cE) +' sE state_tgt).
 
-  Variable world: Type.
-  Variable world_le: world -> world -> Prop.
-
   Definition shared :=
     (TIdSet.t *
        (@imap ident_src wf_src) *
        (@imap ident_tgt wf_tgt) *
        state_src *
        state_tgt *
-       world)%type.
+       URA.car)%type.
 
   Let shared_rel: Type := shared -> Prop.
-
-  Definition shared_rel_wf (r: shared_rel): Prop :=
-    forall ths im_src0 im_tgt0 st_src st_tgt w0
-           (INV: r (ths, im_src0, im_tgt0, st_src, st_tgt, w0))
-           im_tgt1 (TGT: fair_update im_tgt0 im_tgt1 (sum_fmap_l (tids_fmap_all ths))),
-    exists im_src1 w1,
-      (<<SRC: fair_update im_src0 im_src1 (sum_fmap_l (tids_fmap_all ths))>>) /\
-        (<<INV: r (ths, im_src1, im_tgt1, st_src, st_tgt, w1)>>) /\
-        (<<WORLD: world_le w0 w1>>).
 
   Variable I: shared_rel.
 
   Variant __lsim
           (tid: thread_id)
-          (lsim: forall R_src R_tgt (RR: R_src -> R_tgt -> shared_rel), bool -> bool -> itree srcE R_src -> itree tgtE R_tgt -> shared_rel)
-          (_lsim: forall R_src R_tgt (RR: R_src -> R_tgt -> shared_rel),bool -> bool -> itree srcE R_src -> itree tgtE R_tgt -> shared_rel)
-          R_src R_tgt (RR: R_src -> R_tgt -> shared_rel)
+          (lsim: forall R_src R_tgt (RR: R_src -> R_tgt -> URA.car -> URA.car -> shared_rel), bool -> bool -> URA.car -> URA.car -> itree srcE R_src -> itree tgtE R_tgt -> shared_rel)
+          (_lsim: forall R_src R_tgt (RR: R_src -> R_tgt -> URA.car -> URA.car -> shared_rel),bool -> bool -> URA.car -> URA.car -> itree srcE R_src -> itree tgtE R_tgt -> shared_rel)
+          R_src R_tgt (RR: R_src -> R_tgt -> URA.car -> URA.car -> shared_rel)
     :
-    bool -> bool -> itree srcE R_src -> itree tgtE R_tgt -> shared_rel :=
+    bool -> bool -> URA.car -> URA.car -> itree srcE R_src -> itree tgtE R_tgt -> shared_rel :=
   | lsim_ret
-      f_src f_tgt
-      ths im_src im_tgt st_src st_tgt w
+      f_src f_tgt r_own r_ctx
+      ths im_src im_tgt st_src st_tgt r_shared
       r_src r_tgt
-      (LSIM: RR r_src r_tgt (ths, im_src, im_tgt, st_src, st_tgt, w))
+      (LSIM: RR r_src r_tgt r_own r_ctx (ths, im_src, im_tgt, st_src, st_tgt, r_shared))
     :
-    __lsim tid lsim _lsim RR f_src f_tgt (Ret r_src) (Ret r_tgt) (ths, im_src, im_tgt, st_src, st_tgt, w)
+    __lsim tid lsim _lsim RR f_src f_tgt r_own r_ctx (Ret r_src) (Ret r_tgt) (ths, im_src, im_tgt, st_src, st_tgt, r_shared)
 
   | lsim_tauL
-      f_src f_tgt
-      ths im_src im_tgt st_src st_tgt w
+      f_src f_tgt r_own r_ctx
+      ths im_src im_tgt st_src st_tgt r_shared
       itr_src itr_tgt
-      (LSIM: _lsim _ _ RR true f_tgt itr_src itr_tgt (ths, im_src, im_tgt, st_src, st_tgt, w))
+      (LSIM: _lsim _ _ RR true f_tgt r_own r_ctx itr_src itr_tgt (ths, im_src, im_tgt, st_src, st_tgt, r_shared))
     :
-    __lsim tid lsim _lsim RR f_src f_tgt (Tau itr_src) itr_tgt (ths, im_src, im_tgt, st_src, st_tgt, w)
+    __lsim tid lsim _lsim RR f_src f_tgt r_own r_ctx (Tau itr_src) itr_tgt (ths, im_src, im_tgt, st_src, st_tgt, r_shared)
   | lsim_chooseL
-      f_src f_tgt
-      ths im_src im_tgt st_src st_tgt w
+      f_src f_tgt r_own r_ctx
+      ths im_src im_tgt st_src st_tgt r_shared
       X ktr_src itr_tgt
-      (LSIM: exists x, _lsim _ _ RR true f_tgt (ktr_src x) itr_tgt (ths, im_src, im_tgt, st_src, st_tgt, w))
+      (LSIM: exists x, _lsim _ _ RR true f_tgt r_own r_ctx (ktr_src x) itr_tgt (ths, im_src, im_tgt, st_src, st_tgt, r_shared))
     :
-    __lsim tid lsim _lsim RR f_src f_tgt (trigger (Choose X) >>= ktr_src) itr_tgt (ths, im_src, im_tgt, st_src, st_tgt, w)
+    __lsim tid lsim _lsim RR f_src f_tgt r_own r_ctx (trigger (Choose X) >>= ktr_src) itr_tgt (ths, im_src, im_tgt, st_src, st_tgt, r_shared)
   | lsim_putL
-      f_src f_tgt
-      ths im_src im_tgt st_src st_tgt w
+      f_src f_tgt r_own r_ctx
+      ths im_src im_tgt st_src st_tgt r_shared
       st ktr_src itr_tgt
-      (LSIM: _lsim _ _ RR true f_tgt (ktr_src tt) itr_tgt (ths, im_src, im_tgt, st, st_tgt, w))
+      (LSIM: _lsim _ _ RR true f_tgt r_own r_ctx (ktr_src tt) itr_tgt (ths, im_src, im_tgt, st, st_tgt, r_shared))
     :
-    __lsim tid lsim _lsim RR f_src f_tgt (trigger (Put st) >>= ktr_src) itr_tgt (ths, im_src, im_tgt, st_src, st_tgt, w)
+    __lsim tid lsim _lsim RR f_src f_tgt r_own r_ctx (trigger (Put st) >>= ktr_src) itr_tgt (ths, im_src, im_tgt, st_src, st_tgt, r_shared)
   | lsim_getL
-      f_src f_tgt
-      ths im_src im_tgt st_src st_tgt w
+      f_src f_tgt r_own r_ctx
+      ths im_src im_tgt st_src st_tgt r_shared
       ktr_src itr_tgt
-      (LSIM: _lsim _ _ RR true f_tgt (ktr_src st_src) itr_tgt (ths, im_src, im_tgt, st_src, st_tgt, w))
+      (LSIM: _lsim _ _ RR true f_tgt r_own r_ctx (ktr_src st_src) itr_tgt (ths, im_src, im_tgt, st_src, st_tgt, r_shared))
     :
-    __lsim tid lsim _lsim RR f_src f_tgt (trigger (@Get _) >>= ktr_src) itr_tgt (ths, im_src, im_tgt, st_src, st_tgt, w)
+    __lsim tid lsim _lsim RR f_src f_tgt r_own r_ctx (trigger (@Get _) >>= ktr_src) itr_tgt (ths, im_src, im_tgt, st_src, st_tgt, r_shared)
   | lsim_tidL
-      f_src f_tgt
-      ths im_src im_tgt st_src st_tgt w
+      f_src f_tgt r_own r_ctx
+      ths im_src im_tgt st_src st_tgt r_shared
       ktr_src itr_tgt
-      (LSIM: _lsim _ _ RR true f_tgt (ktr_src tid) itr_tgt (ths, im_src, im_tgt, st_src, st_tgt, w))
+      (LSIM: _lsim _ _ RR true f_tgt r_own r_ctx (ktr_src tid) itr_tgt (ths, im_src, im_tgt, st_src, st_tgt, r_shared))
     :
-    __lsim tid lsim _lsim RR f_src f_tgt (trigger (GetTid) >>= ktr_src) itr_tgt (ths, im_src, im_tgt, st_src, st_tgt, w)
+    __lsim tid lsim _lsim RR f_src f_tgt r_own r_ctx (trigger (GetTid) >>= ktr_src) itr_tgt (ths, im_src, im_tgt, st_src, st_tgt, r_shared)
   | lsim_UB
-      f_src f_tgt
-      ths im_src im_tgt st_src st_tgt w
+      f_src f_tgt r_own r_ctx
+      ths im_src im_tgt st_src st_tgt r_shared
       ktr_src itr_tgt
     :
-    __lsim tid lsim _lsim RR f_src f_tgt (trigger (Undefined) >>= ktr_src) itr_tgt (ths, im_src, im_tgt, st_src, st_tgt, w)
+    __lsim tid lsim _lsim RR f_src f_tgt r_own r_ctx (trigger (Undefined) >>= ktr_src) itr_tgt (ths, im_src, im_tgt, st_src, st_tgt, r_shared)
   | lsim_fairL
-      f_src f_tgt
-      ths im_src0 im_tgt st_src st_tgt w
+      f_src f_tgt r_own r_ctx
+      ths im_src0 im_tgt st_src st_tgt r_shared
       f ktr_src itr_tgt
       (LSIM: exists im_src1,
           (<<FAIR: fair_update im_src0 im_src1 (sum_fmap_r f)>>) /\
-            (<<LSIM: _lsim _ _ RR true f_tgt (ktr_src tt) itr_tgt (ths, im_src1, im_tgt, st_src, st_tgt, w)>>))
+            (<<LSIM: _lsim _ _ RR true f_tgt r_own r_ctx (ktr_src tt) itr_tgt (ths, im_src1, im_tgt, st_src, st_tgt, r_shared)>>))
     :
-    __lsim tid lsim _lsim RR f_src f_tgt (trigger (Fair f) >>= ktr_src) itr_tgt (ths, im_src0, im_tgt, st_src, st_tgt, w)
+    __lsim tid lsim _lsim RR f_src f_tgt r_own r_ctx (trigger (Fair f) >>= ktr_src) itr_tgt (ths, im_src0, im_tgt, st_src, st_tgt, r_shared)
 
   | lsim_tauR
-      f_src f_tgt
-      ths im_src im_tgt st_src st_tgt w
+      f_src f_tgt r_own r_ctx
+      ths im_src im_tgt st_src st_tgt r_shared
       itr_src itr_tgt
-      (LSIM: _lsim _ _ RR f_src true itr_src itr_tgt (ths, im_src, im_tgt, st_src, st_tgt, w))
+      (LSIM: _lsim _ _ RR f_src true r_own r_ctx itr_src itr_tgt (ths, im_src, im_tgt, st_src, st_tgt, r_shared))
     :
-    __lsim tid lsim _lsim RR f_src f_tgt itr_src (Tau itr_tgt) (ths, im_src, im_tgt, st_src, st_tgt, w)
+    __lsim tid lsim _lsim RR f_src f_tgt r_own r_ctx itr_src (Tau itr_tgt) (ths, im_src, im_tgt, st_src, st_tgt, r_shared)
   | lsim_chooseR
-      f_src f_tgt
-      ths im_src im_tgt st_src st_tgt w
+      f_src f_tgt r_own r_ctx
+      ths im_src im_tgt st_src st_tgt r_shared
       X itr_src ktr_tgt
-      (LSIM: forall x, _lsim _ _ RR f_src true itr_src (ktr_tgt x) (ths, im_src, im_tgt, st_src, st_tgt, w))
+      (LSIM: forall x, _lsim _ _ RR f_src true r_own r_ctx itr_src (ktr_tgt x) (ths, im_src, im_tgt, st_src, st_tgt, r_shared))
     :
-    __lsim tid lsim _lsim RR f_src f_tgt itr_src (trigger (Choose X) >>= ktr_tgt) (ths, im_src, im_tgt, st_src, st_tgt, w)
+    __lsim tid lsim _lsim RR f_src f_tgt r_own r_ctx itr_src (trigger (Choose X) >>= ktr_tgt) (ths, im_src, im_tgt, st_src, st_tgt, r_shared)
   | lsim_putR
-      f_src f_tgt
-      ths im_src im_tgt st_src st_tgt w
+      f_src f_tgt r_own r_ctx
+      ths im_src im_tgt st_src st_tgt r_shared
       st itr_src ktr_tgt
-      (LSIM: _lsim _ _ RR f_src true itr_src (ktr_tgt tt) (ths, im_src, im_tgt, st_src, st, w))
+      (LSIM: _lsim _ _ RR f_src true r_own r_ctx itr_src (ktr_tgt tt) (ths, im_src, im_tgt, st_src, st, r_shared))
     :
-    __lsim tid lsim _lsim RR f_src f_tgt itr_src (trigger (Put st) >>= ktr_tgt) (ths, im_src, im_tgt, st_src, st_tgt, w)
+    __lsim tid lsim _lsim RR f_src f_tgt r_own r_ctx itr_src (trigger (Put st) >>= ktr_tgt) (ths, im_src, im_tgt, st_src, st_tgt, r_shared)
   | lsim_getR
-      f_src f_tgt
-      ths im_src im_tgt st_src st_tgt w
+      f_src f_tgt r_own r_ctx
+      ths im_src im_tgt st_src st_tgt r_shared
       itr_src ktr_tgt
-      (LSIM: _lsim _ _ RR f_src true itr_src (ktr_tgt st_tgt) (ths, im_src, im_tgt, st_src, st_tgt, w))
+      (LSIM: _lsim _ _ RR f_src true r_own r_ctx itr_src (ktr_tgt st_tgt) (ths, im_src, im_tgt, st_src, st_tgt, r_shared))
     :
-    __lsim tid lsim _lsim RR f_src f_tgt itr_src (trigger (@Get _) >>= ktr_tgt) (ths, im_src, im_tgt, st_src, st_tgt, w)
+    __lsim tid lsim _lsim RR f_src f_tgt r_own r_ctx itr_src (trigger (@Get _) >>= ktr_tgt) (ths, im_src, im_tgt, st_src, st_tgt, r_shared)
   | lsim_tidR
-      f_src f_tgt
-      ths im_src im_tgt st_src st_tgt w
+      f_src f_tgt r_own r_ctx
+      ths im_src im_tgt st_src st_tgt r_shared
       itr_src ktr_tgt
-      (LSIM: _lsim _ _ RR f_src true itr_src (ktr_tgt tid) (ths, im_src, im_tgt, st_src, st_tgt, w))
+      (LSIM: _lsim _ _ RR f_src true r_own r_ctx itr_src (ktr_tgt tid) (ths, im_src, im_tgt, st_src, st_tgt, r_shared))
     :
-    __lsim tid lsim _lsim RR f_src f_tgt itr_src (trigger (GetTid) >>= ktr_tgt) (ths, im_src, im_tgt, st_src, st_tgt, w)
+    __lsim tid lsim _lsim RR f_src f_tgt r_own r_ctx itr_src (trigger (GetTid) >>= ktr_tgt) (ths, im_src, im_tgt, st_src, st_tgt, r_shared)
   | lsim_fairR
-      f_src f_tgt
-      ths im_src im_tgt0 st_src st_tgt w
+      f_src f_tgt r_own r_ctx
+      ths im_src im_tgt0 st_src st_tgt r_shared
       f itr_src ktr_tgt
       (LSIM: forall im_tgt1
                    (FAIR: fair_update im_tgt0 im_tgt1 (sum_fmap_r f)),
-          (<<LSIM: _lsim _ _ RR f_src true itr_src (ktr_tgt tt) (ths, im_src, im_tgt1, st_src, st_tgt, w)>>))
+          (<<LSIM: _lsim _ _ RR f_src true r_own r_ctx itr_src (ktr_tgt tt) (ths, im_src, im_tgt1, st_src, st_tgt, r_shared)>>))
     :
-    __lsim tid lsim _lsim RR f_src f_tgt itr_src (trigger (Fair f) >>= ktr_tgt) (ths, im_src, im_tgt0, st_src, st_tgt, w)
+    __lsim tid lsim _lsim RR f_src f_tgt r_own r_ctx itr_src (trigger (Fair f) >>= ktr_tgt) (ths, im_src, im_tgt0, st_src, st_tgt, r_shared)
 
   | lsim_observe
-      f_src f_tgt
-      ths im_src im_tgt st_src st_tgt w
+      f_src f_tgt r_own r_ctx
+      ths im_src im_tgt st_src st_tgt r_shared
       fn args ktr_src ktr_tgt
       (LSIM: forall ret,
-          lsim _ _ RR true true (ktr_src ret) (ktr_tgt ret) (ths, im_src, im_tgt, st_src, st_tgt, w))
+          lsim _ _ RR true true r_own r_ctx (ktr_src ret) (ktr_tgt ret) (ths, im_src, im_tgt, st_src, st_tgt, r_shared))
     :
-    __lsim tid lsim _lsim RR f_src f_tgt (trigger (Observe fn args) >>= ktr_src) (trigger (Observe fn args) >>= ktr_tgt) (ths, im_src, im_tgt, st_src, st_tgt, w)
+    __lsim tid lsim _lsim RR f_src f_tgt r_own r_ctx (trigger (Observe fn args) >>= ktr_src) (trigger (Observe fn args) >>= ktr_tgt) (ths, im_src, im_tgt, st_src, st_tgt, r_shared)
 
   | lsim_sync
-      f_src f_tgt
-      ths0 im_src0 im_tgt0 st_src0 st_tgt0 w
-      w0 ktr_src ktr_tgt
-      (INV: I (ths0, im_src0, im_tgt0, st_src0, st_tgt0, w0))
-      (WORLD: world_le w w0)
-      (LSIM: forall ths1 im_src1 im_tgt1 st_src1 st_tgt1 w1
-                   (INV: I (ths1, im_src1, im_tgt1, st_src1, st_tgt1, w1))
-                   (WORLD: world_le w0 w1)
-                   im_tgt2
-                   (TGT: fair_update im_tgt1 im_tgt2 (sum_fmap_l (tids_fmap tid ths1))),
-          _lsim _ _ RR f_src true (trigger (Yield) >>= ktr_src) (ktr_tgt tt) (ths1, im_src1, im_tgt2, st_src1, st_tgt1, w1))
+      f_src f_tgt r_own0 r_ctx0
+      ths0 im_src0 im_tgt0 st_src0 st_tgt0 r_shared0
+      r_own1 ktr_src ktr_tgt
+      (INV: I (ths0, im_src0, im_tgt0, st_src0, st_tgt0, r_shared0))
+      (VALID: URA.wf (r_shared0 ⋅ r_own0 ⋅ r_ctx0))
+      (LSIM: forall ths1 im_src1 im_tgt1 st_src1 st_tgt1 r_shared1 r_ctx1
+                    (INV: I (ths1, im_src1, im_tgt1, st_src1, st_tgt1, r_shared1))
+                    (VALID: URA.wf (r_shared1 ⋅ r_own0 ⋅ r_ctx1))
+                    im_tgt2
+                    (TGT: fair_update im_tgt1 im_tgt2 (sum_fmap_l (tids_fmap tid ths1))),
+          _lsim _ _ RR f_src true r_own1 r_ctx1 (trigger (Yield) >>= ktr_src) (ktr_tgt tt) (ths1, im_src1, im_tgt2, st_src1, st_tgt1, r_shared1))
     :
-    __lsim tid lsim _lsim RR f_src f_tgt (trigger (Yield) >>= ktr_src) (trigger (Yield) >>= ktr_tgt) (ths0, im_src0, im_tgt0, st_src0, st_tgt0, w)
+    __lsim tid lsim _lsim RR f_src f_tgt r_own0 r_ctx0 (trigger (Yield) >>= ktr_src) (trigger (Yield) >>= ktr_tgt) (ths0, im_src0, im_tgt0, st_src0, st_tgt0, r_shared0)
   | lsim_yieldL
-      f_src f_tgt
-      ths im_src0 im_tgt st_src st_tgt w
+      f_src f_tgt r_own r_ctx
+      ths im_src0 im_tgt st_src st_tgt r_shared
       ktr_src itr_tgt
       (LSIM: exists im_src1,
           (<<FAIR: fair_update im_src0 im_src1 (sum_fmap_l (tids_fmap tid ths))>>) /\
-            (<<LSIM: _lsim _ _ RR true f_tgt (ktr_src tt) itr_tgt (ths, im_src1, im_tgt, st_src, st_tgt, w)>>))
+            (<<LSIM: _lsim _ _ RR true f_tgt r_own r_ctx (ktr_src tt) itr_tgt (ths, im_src1, im_tgt, st_src, st_tgt, r_shared)>>))
     :
-    __lsim tid lsim _lsim RR f_src f_tgt (trigger (Yield) >>= ktr_src) itr_tgt (ths, im_src0, im_tgt, st_src, st_tgt, w)
+    __lsim tid lsim _lsim RR f_src f_tgt r_own r_ctx (trigger (Yield) >>= ktr_src) itr_tgt (ths, im_src0, im_tgt, st_src, st_tgt, r_shared)
 
   | lsim_progress
-      ths im_src im_tgt st_src st_tgt w
+      r_own r_ctx
+      ths im_src im_tgt st_src st_tgt r_shared
       itr_src itr_tgt
-      (LSIM: lsim _ _ RR false false itr_src itr_tgt (ths, im_src, im_tgt, st_src, st_tgt, w))
+      (LSIM: lsim _ _ RR false false r_own r_ctx itr_src itr_tgt (ths, im_src, im_tgt, st_src, st_tgt, r_shared))
     :
-    __lsim tid lsim _lsim RR true true itr_src itr_tgt (ths, im_src, im_tgt, st_src, st_tgt, w)
+    __lsim tid lsim _lsim RR true true r_own r_ctx itr_src itr_tgt (ths, im_src, im_tgt, st_src, st_tgt, r_shared)
   .
 
   Definition lsim (tid: thread_id)
-             R_src R_tgt (RR: R_src -> R_tgt -> shared_rel):
-    bool -> bool -> itree srcE R_src -> itree tgtE R_tgt -> shared_rel :=
-    paco8 (fun r => pind8 (__lsim tid r) top8) bot8 R_src R_tgt RR.
+             R_src R_tgt (RR: R_src -> R_tgt -> URA.car -> URA.car -> shared_rel):
+    bool -> bool -> URA.car -> URA.car -> itree srcE R_src -> itree tgtE R_tgt -> shared_rel :=
+    paco10 (fun r => pind10 (__lsim tid r) top10) bot10 R_src R_tgt RR.
 
   Lemma __lsim_mon tid:
-    forall r r' (LE: r <8= r'), (__lsim tid r) <9= (__lsim tid r').
+    forall r r' (LE: r <10= r'), (__lsim tid r) <11= (__lsim tid r').
   Proof.
     ii. inv PR; econs; eauto.
   Qed.
 
-  Lemma _lsim_mon tid: forall r, monotone8 (__lsim tid r).
+  Lemma _lsim_mon tid: forall r, monotone10 (__lsim tid r).
   Proof.
     ii. inv IN; econs; eauto.
     { des. eauto. }
@@ -221,129 +213,129 @@ Section PRIMIVIESIM.
     { des. esplits; eauto. }
   Qed.
 
-  Lemma lsim_mon tid: forall q, monotone8 (fun r => pind8 (__lsim tid r) q).
+  Lemma lsim_mon tid: forall q, monotone10 (fun r => pind10 (__lsim tid r) q).
   Proof.
-    ii. eapply pind8_mon_gen; eauto.
+    ii. eapply pind10_mon_gen; eauto.
     ii. eapply __lsim_mon; eauto.
   Qed.
 
   Variant lsim_resetC
-          (r: forall R_src R_tgt (RR: R_src -> R_tgt -> shared_rel), bool -> bool -> itree srcE R_src -> itree tgtE R_tgt -> shared_rel)
-          R_src R_tgt (RR: R_src -> R_tgt -> shared_rel)
+          (r: forall R_src R_tgt (RR: R_src -> R_tgt -> URA.car -> URA.car -> shared_rel), bool -> bool -> URA.car -> URA.car -> itree srcE R_src -> itree tgtE R_tgt -> shared_rel)
+          R_src R_tgt (RR: R_src -> R_tgt -> URA.car -> URA.car -> shared_rel)
     :
-    bool -> bool -> itree srcE R_src -> itree tgtE R_tgt -> shared_rel :=
+    bool -> bool -> URA.car -> URA.car -> itree srcE R_src -> itree tgtE R_tgt -> shared_rel :=
     | lsim_resetC_intro
-        src tgt shr
+        src tgt shr r_own r_ctx
         ps0 pt0 ps1 pt1
-        (REL: r _ _ RR ps1 pt1 src tgt shr)
+        (REL: r _ _ RR ps1 pt1 r_own r_ctx src tgt shr)
         (SRC: ps1 = true -> ps0 = true)
         (TGT: pt1 = true -> pt0 = true)
       :
-      lsim_resetC r RR ps0 pt0 src tgt shr
+      lsim_resetC r RR ps0 pt0 r_own r_ctx src tgt shr
   .
 
   Lemma lsim_resetC_spec tid
     :
-    lsim_resetC <9= gupaco8 (fun r => pind8 (__lsim tid r) top8) (cpn8 (fun r => pind8 (__lsim tid r) top8)).
+    lsim_resetC <11= gupaco10 (fun r => pind10 (__lsim tid r) top10) (cpn10 (fun r => pind10 (__lsim tid r) top10)).
   Proof.
-    eapply wrespect8_uclo; eauto with paco.
+    eapply wrespect10_uclo; eauto with paco.
     { eapply lsim_mon. }
     econs.
     { ii. inv IN. econs; eauto. }
     i. inv PR. eapply GF in REL.
-    eapply pind8_acc in REL.
-    instantiate (1:= (fun R0 R1 (RR: R0 -> R1 -> shared_rel) ps1 pt1 src tgt shr =>
+    eapply pind10_acc in REL.
+    instantiate (1:= (fun R0 R1 (RR: R0 -> R1 -> URA.car -> URA.car -> shared_rel) ps1 pt1 r_own r_ctx src tgt shr =>
                         forall ps0 pt0,
                           (ps1 = true -> ps0 = true) ->
                           (pt1 = true -> pt0 = true) ->
-                          pind8 (__lsim tid (rclo8 lsim_resetC r)) top8 R0 R1 RR ps0 pt0 src tgt shr)) in REL; eauto.
-    ss. i. eapply pind8_unfold in PR.
+                          pind10 (__lsim tid (rclo10 lsim_resetC r)) top10 R0 R1 RR ps0 pt0 r_own r_ctx src tgt shr)) in REL; eauto.
+    ss. i. eapply pind10_unfold in PR.
     2:{ eapply _lsim_mon. }
     rename PR into LSIM. inv LSIM.
 
-    { eapply pind8_fold. econs; eauto. }
+    { eapply pind10_fold. econs; eauto. }
 
     { destruct LSIM0 as [LSIM0 IND]. clear LSIM0.
-      eapply pind8_fold. eapply lsim_tauL. split; ss.
+      eapply pind10_fold. eapply lsim_tauL. split; ss.
       hexploit IH; eauto.
     }
 
-    { des. eapply pind8_fold. eapply lsim_chooseL. esplits; eauto. split; ss.
+    { des. eapply pind10_fold. eapply lsim_chooseL. esplits; eauto. split; ss.
       destruct LSIM0 as [LSIM0 IND]. hexploit IH; eauto.
     }
 
-    { eapply pind8_fold. eapply lsim_putL. split; ss.
+    { eapply pind10_fold. eapply lsim_putL. split; ss.
       destruct LSIM0 as [LSIM0 IND]. hexploit IH; eauto.
     }
 
-    { eapply pind8_fold. eapply lsim_getL. split; ss.
+    { eapply pind10_fold. eapply lsim_getL. split; ss.
       destruct LSIM0 as [LSIM0 IND]. hexploit IH; eauto.
     }
 
-    { eapply pind8_fold. eapply lsim_tidL. split; ss.
+    { eapply pind10_fold. eapply lsim_tidL. split; ss.
       destruct LSIM0 as [LSIM0 IND]. hexploit IH; eauto.
     }
 
-    { eapply pind8_fold. eapply lsim_UB. }
+    { eapply pind10_fold. eapply lsim_UB. }
 
-    { des. eapply pind8_fold. eapply lsim_fairL. esplits; eauto. split; ss.
+    { des. eapply pind10_fold. eapply lsim_fairL. esplits; eauto. split; ss.
       destruct LSIM as [LSIM IND]. hexploit IH; eauto.
     }
 
     { destruct LSIM0 as [LSIM0 IND]. clear LSIM0.
-      eapply pind8_fold. eapply lsim_tauR. split; ss.
+      eapply pind10_fold. eapply lsim_tauR. split; ss.
       hexploit IH. eauto. all: eauto.
     }
 
-    { eapply pind8_fold. eapply lsim_chooseR. i. split; ss. specialize (LSIM0 x).
+    { eapply pind10_fold. eapply lsim_chooseR. i. split; ss. specialize (LSIM0 x).
       destruct LSIM0 as [LSIM0 IND]. hexploit IH; eauto.
     }
 
-    { eapply pind8_fold. eapply lsim_putR. split; ss.
+    { eapply pind10_fold. eapply lsim_putR. split; ss.
       destruct LSIM0 as [LSIM0 IND]. hexploit IH; eauto.
     }
 
-    { eapply pind8_fold. eapply lsim_getR. split; ss.
+    { eapply pind10_fold. eapply lsim_getR. split; ss.
       destruct LSIM0 as [LSIM0 IND]. hexploit IH; eauto.
     }
 
-    { eapply pind8_fold. eapply lsim_tidR. split; ss.
+    { eapply pind10_fold. eapply lsim_tidR. split; ss.
       destruct LSIM0 as [LSIM0 IND]. hexploit IH; eauto.
     }
 
-    { eapply pind8_fold. eapply lsim_fairR. i. split; ss. specialize (LSIM0 _ FAIR).
+    { eapply pind10_fold. eapply lsim_fairR. i. split; ss. specialize (LSIM0 _ FAIR).
       des. destruct LSIM0 as [LSIM0 IND]. hexploit IH; eauto.
     }
 
-    { eapply pind8_fold. eapply lsim_observe. i. eapply rclo8_base. auto. }
+    { eapply pind10_fold. eapply lsim_observe. i. eapply rclo10_base. auto. }
 
-    { eapply pind8_fold. eapply lsim_sync; eauto. i.
+    { eapply pind10_fold. eapply lsim_sync; eauto. i.
       hexploit LSIM0; eauto. clear LSIM0. intros LSIM0.
-      destruct LSIM0 as [LSIM0 IND]. hexploit IH; eauto. i. split; ss.
+      destruct LSIM0 as [LSIM0 IND]. hexploit IH; eauto. i. split; ss; eauto.
     }
 
-    { des. eapply pind8_fold. eapply lsim_yieldL. esplits; eauto. split; ss.
+    { des. eapply pind10_fold. eapply lsim_yieldL. esplits; eauto. split; ss.
       destruct LSIM as [LSIM IND]. hexploit IH; eauto.
     }
 
     { pclearbot. hexploit H; ss; i. hexploit H0; ss; i. clarify.
-      eapply pind8_fold. eapply lsim_progress. eapply rclo8_base. auto. }
+      eapply pind10_fold. eapply lsim_progress. eapply rclo10_base. auto. }
   Qed.
 
   Lemma lsim_reset_prog
         tid
-        R0 R1 (RR: R0 -> R1 -> shared_rel)
+        R0 R1 (RR: R0 -> R1 -> URA.car -> URA.car -> shared_rel)
         src tgt shr
-        ps0 pt0 ps1 pt1
-        (LSIM: lsim tid RR ps1 pt1 src tgt shr)
+        ps0 pt0 ps1 pt1 r_own r_ctx
+        (LSIM: lsim tid RR ps1 pt1 r_own r_ctx src tgt shr)
         (SRC: ps1 = true -> ps0 = true)
         (TGT: pt1 = true -> pt0 = true)
     :
-    lsim tid RR ps0 pt0 src tgt shr.
+    lsim tid RR ps0 pt0 r_own r_ctx src tgt shr.
   Proof.
     ginit.
     { eapply lsim_mon. }
-    { eapply cpn8_wcompat. eapply lsim_mon. }
+    { eapply cpn10_wcompat. eapply lsim_mon. }
     guclo lsim_resetC_spec.
     { eapply lsim_mon. }
     econs; eauto. gfinal.
@@ -353,132 +345,146 @@ Section PRIMIVIESIM.
 
   Lemma lsim_set_prog
         tid
-        R0 R1 (RR: R0 -> R1 -> shared_rel)
-        src tgt shr
-        (LSIM: lsim tid RR true true src tgt shr)
+        R0 R1 (RR: R0 -> R1 -> URA.car -> URA.car -> shared_rel)
+        r_own r_ctx src tgt shr
+        (LSIM: lsim tid RR true true r_own r_ctx src tgt shr)
     :
-    forall ps pt, lsim tid RR ps pt src tgt shr.
+    forall ps pt, lsim tid RR ps pt r_own r_ctx src tgt shr.
   Proof.
     i. revert_until tid. pcofix CIH. i.
     remember true as ps0 in LSIM at 1. remember true as pt0 in LSIM at 1.
     move LSIM before CIH. revert_until LSIM. punfold LSIM.
     2:{ eapply lsim_mon. }
-    eapply pind8_acc in LSIM.
+    eapply pind10_acc in LSIM.
 
-    { instantiate (1:= (fun R0 R1 (RR: R0 -> R1 -> shared_rel) ps0 pt0 src tgt shr =>
+    { instantiate (1:= (fun R0 R1 (RR: R0 -> R1 -> URA.car -> URA.car -> shared_rel) ps0 pt0 r_own r_ctx src tgt shr =>
                           ps0 = true ->
                           pt0 = true ->
                           forall ps pt,
-                            paco8
+                            paco10
                               (fun r0 =>
-                                 pind8 (__lsim tid r0) top8) r R0 R1 RR ps pt src tgt shr)) in LSIM; auto. }
+                                 pind10 (__lsim tid r0) top10) r R0 R1 RR ps pt r_own r_ctx src tgt shr)) in LSIM; auto. }
 
-    ss. clear ps0 pt0 src tgt shr LSIM.
-    intros rr DEC IH R0' R1' RR' gps gpt src tgt shr LSIM. clear DEC.
+    ss. clear ps0 pt0 r_own r_ctx src tgt shr LSIM.
+    intros rr DEC IH R0' R1' RR' gps gpt r_own r_ctx src tgt shr LSIM. clear DEC.
     intros Egps Egpt ps pt.
-    eapply pind8_unfold in LSIM.
+    eapply pind10_unfold in LSIM.
     2:{ eapply _lsim_mon. }
     inv LSIM.
 
-    { pfold. eapply pind8_fold. econs; eauto. }
+    { pfold. eapply pind10_fold. econs; eauto. }
 
     { destruct LSIM0 as [LSIM0 IND]. clear LSIM0.
-      pfold. eapply pind8_fold. eapply lsim_tauL. split; ss.
+      pfold. eapply pind10_fold. eapply lsim_tauL. split; ss.
       hexploit IH. eauto. all: eauto. i. punfold H. eapply lsim_mon.
     }
 
-    { des. pfold. eapply pind8_fold. eapply lsim_chooseL. esplits; eauto. split; ss.
+    { des. pfold. eapply pind10_fold. eapply lsim_chooseL. esplits; eauto. split; ss.
       destruct LSIM0 as [LSIM0 IND]. hexploit IH; eauto. i. punfold H. eapply lsim_mon.
     }
 
-    { pfold. eapply pind8_fold. eapply lsim_putL. split; ss.
+    { pfold. eapply pind10_fold. eapply lsim_putL. split; ss.
       destruct LSIM0 as [LSIM0 IND]. hexploit IH; eauto. i. punfold H. eapply lsim_mon.
     }
 
-    { pfold. eapply pind8_fold. eapply lsim_getL. split; ss.
+    { pfold. eapply pind10_fold. eapply lsim_getL. split; ss.
       destruct LSIM0 as [LSIM0 IND]. hexploit IH; eauto. i. punfold H. eapply lsim_mon.
     }
 
-    { pfold. eapply pind8_fold. eapply lsim_tidL. split; ss.
+    { pfold. eapply pind10_fold. eapply lsim_tidL. split; ss.
       destruct LSIM0 as [LSIM0 IND]. hexploit IH; eauto. i. punfold H. eapply lsim_mon.
     }
 
-    { pfold. eapply pind8_fold. eapply lsim_UB. }
+    { pfold. eapply pind10_fold. eapply lsim_UB. }
 
-    { des. pfold. eapply pind8_fold. eapply lsim_fairL. esplits; eauto. split; ss.
+    { des. pfold. eapply pind10_fold. eapply lsim_fairL. esplits; eauto. split; ss.
       destruct LSIM as [LSIM IND]. hexploit IH; eauto. i. punfold H. eapply lsim_mon.
     }
 
     { destruct LSIM0 as [LSIM0 IND]. clear LSIM0.
-      pfold. eapply pind8_fold. eapply lsim_tauR. split; ss.
+      pfold. eapply pind10_fold. eapply lsim_tauR. split; ss.
       hexploit IH. eauto. all: eauto. i. punfold H. eapply lsim_mon.
     }
 
-    { pfold. eapply pind8_fold. eapply lsim_chooseR. i. split; ss. specialize (LSIM0 x).
+    { pfold. eapply pind10_fold. eapply lsim_chooseR. i. split; ss. specialize (LSIM0 x).
       destruct LSIM0 as [LSIM0 IND]. hexploit IH; eauto. i. punfold H. eapply lsim_mon.
     }
 
-    { pfold. eapply pind8_fold. eapply lsim_putR. split; ss.
+    { pfold. eapply pind10_fold. eapply lsim_putR. split; ss.
       destruct LSIM0 as [LSIM0 IND]. hexploit IH; eauto. i. punfold H. eapply lsim_mon.
     }
 
-    { pfold. eapply pind8_fold. eapply lsim_getR. split; ss.
+    { pfold. eapply pind10_fold. eapply lsim_getR. split; ss.
       destruct LSIM0 as [LSIM0 IND]. hexploit IH; eauto. i. punfold H. eapply lsim_mon.
     }
 
-    { pfold. eapply pind8_fold. eapply lsim_tidR. split; ss.
+    { pfold. eapply pind10_fold. eapply lsim_tidR. split; ss.
       destruct LSIM0 as [LSIM0 IND]. hexploit IH; eauto. i. punfold H. eapply lsim_mon.
     }
 
-    { pfold. eapply pind8_fold. eapply lsim_fairR. i. split; ss. specialize (LSIM0 _ FAIR).
+    { pfold. eapply pind10_fold. eapply lsim_fairR. i. split; ss. specialize (LSIM0 _ FAIR).
       des. destruct LSIM0 as [LSIM0 IND]. hexploit IH; eauto. i. punfold H. eapply lsim_mon.
     }
 
-    { pfold. eapply pind8_fold. eapply lsim_observe. i. eapply upaco8_mon_bot; eauto. }
+    { pfold. eapply pind10_fold. eapply lsim_observe. i. eapply upaco10_mon_bot; eauto. }
 
-    { pfold. eapply pind8_fold. eapply lsim_sync; eauto. i.
+    { pfold. eapply pind10_fold. eapply lsim_sync; eauto. i.
       hexploit LSIM0; eauto. clear LSIM0. intros LSIM0.
       destruct LSIM0 as [LSIM0 IND]. hexploit IH; eauto. i. split; ss. punfold H. eapply lsim_mon.
     }
 
-    { des. pfold. eapply pind8_fold. eapply lsim_yieldL. esplits; eauto. split; ss.
+    { des. pfold. eapply pind10_fold. eapply lsim_yieldL. esplits; eauto. split; ss.
       destruct LSIM as [LSIM IND]. hexploit IH; eauto. i. punfold H. eapply lsim_mon.
     }
 
-    { pclearbot. eapply paco8_mon_bot. eapply lsim_reset_prog. eauto. all: ss. }
+    { pclearbot. eapply paco10_mon_bot. eapply lsim_reset_prog. eauto. all: ss. }
 
   Qed.
 
-  Definition local_RR {R0 R1} (RR: R0 -> R1 -> Prop) tid :=
-    fun (r_src: R0) (r_tgt: R1) '(ths2, im_src1, im_tgt1, st_src1, st_tgt1, w1) =>
-      (exists ths3 w2,
+  Definition local_RR {R0 R1} (RR: R0 -> R1 -> Prop) tid:
+    R0 -> R1 -> URA.car -> URA.car -> shared_rel :=
+    fun (r_src: R0) (r_tgt: R1) (r_own1: URA.car) (r_ctx: URA.car) '(ths2, im_src1, im_tgt1, st_src1, st_tgt1, r_shared1) =>
+      (exists ths3 r_own2 r_shared2,
           (<<THS: NatMap.remove tid ths2 = ths3>>) /\
-            (<<WORLD: world_le w1 w2>>) /\
-            (<<INV: I (ths3, im_src1, im_tgt1, st_src1, st_tgt1, w2)>>) /\
+            (<<VALID: URA.wf (r_shared2 ⋅ r_own2 ⋅ r_ctx)>>) /\
+            (<<INV: I (ths3, im_src1, im_tgt1, st_src1, st_tgt1, r_shared2)>>) /\
             (<<RET: RR r_src r_tgt>>)).
 
   Definition local_sim {R0 R1} (RR: R0 -> R1 -> Prop) src tgt :=
-    forall ths0 im_src0 im_tgt0 st_src0 st_tgt0 w0
-           (INV: I (ths0, im_src0, im_tgt0, st_src0, st_tgt0, w0))
+    forall ths0 im_src0 im_tgt0 st_src0 st_tgt0 r_shared0 r_ctx0
+           (INV: I (ths0, im_src0, im_tgt0, st_src0, st_tgt0, r_shared0))
            tid ths1
-           (THS: TIdSet.add_new tid ths0 ths1),
-    exists w1, (<<INV: I (ths1, im_src0, im_tgt0, st_src0, st_tgt0, w1)>>) /\
-                 (<<WORLD: world_le w0 w1>>) /\
-                 (forall ths im_src1 im_tgt1 st_src st_tgt w2
-                         (INV: I (ths, im_src1, im_tgt1, st_src, st_tgt, w2))
-                         (WORLD: world_le w1 w2),
-                   forall im_tgt2 (TGT: fair_update im_tgt1 im_tgt2 (sum_fmap_l (tids_fmap tid ths))),
-                   exists im_src2 w3,
-                     (<<SRC: fair_update im_src1 im_src2 (sum_fmap_l (tids_fmap tid ths))>>) /\
-                       (<<WORLD: world_le w2 w3>>) /\
-                       (<<LSIM: forall fs ft,
-                           lsim
-                             tid
-                             (@local_RR R0 R1 RR tid)
-                             fs ft
-                             src tgt
-                             (ths, im_src2, im_tgt2, st_src, st_tgt, w3)
-                             >>)).
+           (THS: TIdSet.add_new tid ths0 ths1)
+           (VALID: URA.wf (r_shared0 ⋅ r_ctx0)),
+    exists r_shared1 r_own1,
+      (<<INV: I (ths1, im_src0, im_tgt0, st_src0, st_tgt0, r_shared1)>>) /\
+        (<<VALID: URA.wf (r_shared1 ⋅ r_own1 ⋅ r_ctx0)>>) /\
+        (forall ths im_src1 im_tgt1 st_src st_tgt r_shared2 r_ctx2
+                (INV: I (ths, im_src1, im_tgt1, st_src, st_tgt, r_shared2))
+                (VALID: URA.wf (r_shared2 ⋅ r_own1 ⋅ r_ctx2)),
+          forall im_tgt2 (TGT: fair_update im_tgt1 im_tgt2 (sum_fmap_l (tids_fmap tid ths))),
+          exists im_src2,
+            (<<SRC: fair_update im_src1 im_src2 (sum_fmap_l (tids_fmap tid ths))>>) /\
+              (<<LSIM: forall fs ft,
+                  lsim
+                    tid
+                    (@local_RR R0 R1 RR tid)
+                    fs ft
+                    r_own1 r_ctx2
+                    src tgt
+                    (ths, im_src2, im_tgt2, st_src, st_tgt, r_shared2)
+                    >>)).
+
+  Definition shared_rel_wf (r: shared_rel): Prop :=
+    forall ths im_src0 im_tgt0 st_src st_tgt r_shared0 r_ctx
+           (INV: r (ths, im_src0, im_tgt0, st_src, st_tgt, r_shared0))
+           (VALID: URA.wf (r_shared0 ⋅ r_ctx)),
+    forall im_tgt1
+           (TGT: fair_update im_tgt0 im_tgt1 (sum_fmap_l (tids_fmap_all ths))),
+    exists im_src1 r_shared1,
+      (<<SRC: fair_update im_src0 im_src1 (sum_fmap_l (tids_fmap_all ths))>>) /\
+        (<<INV: r (ths, im_src1, im_tgt1, st_src, st_tgt, r_shared1)>>) /\
+        (<<VALID: URA.wf (r_shared1 ⋅ r_ctx)>>).
 
 End PRIMIVIESIM.
 #[export] Hint Constructors __lsim: core.
@@ -486,7 +492,7 @@ End PRIMIVIESIM.
 #[export] Hint Resolve __lsim_mon: paco.
 #[export] Hint Resolve _lsim_mon: paco.
 #[export] Hint Resolve lsim_mon: paco.
-#[export] Hint Resolve cpn5_wcompat: paco.
+
 
 
 Module ModSim.
@@ -502,20 +508,17 @@ Module ModSim.
           wf_tgt_inhabited: inhabited wf_tgt.(T);
           wf_tgt_open: forall (o0: wf_tgt.(T)), exists o1, wf_tgt.(lt) o0 o1;
 
-          world: Type;
-          world_le: world -> world -> Prop;
-          world_le_PreOrder: PreOrder world_le;
+          world: URA.t;
 
-          I: (@shared md_src.(Mod.state) md_tgt.(Mod.state) md_src.(Mod.ident) md_tgt.(Mod.ident) wf_src wf_tgt world) -> Prop;
-
-          init: forall im_tgt, exists im_src w,
-            I (NatSet.empty, im_src, im_tgt, md_src.(Mod.st_init), md_tgt.(Mod.st_init), w);
+          I: (@shared world md_src.(Mod.state) md_tgt.(Mod.state) md_src.(Mod.ident) md_tgt.(Mod.ident) wf_src wf_tgt) -> Prop;
+          init: forall im_tgt, exists im_src r_shared,
+            I (NatSet.empty, im_src, im_tgt, md_src.(Mod.st_init), md_tgt.(Mod.st_init), r_shared);
 
           funs: forall fn args, match md_src.(Mod.funs) fn, md_tgt.(Mod.funs) fn with
-                           | None, _ => True
-                           | _, None => False
-                           | Some ktr_src, Some ktr_tgt => local_sim world_le I (@eq Val) (ktr_src args) (ktr_tgt args)
-                           end;
+                                | None, _ => True
+                                | _, None => False
+                                | Some ktr_src, Some ktr_tgt => local_sim I (@eq Val) (ktr_src args) (ktr_tgt args)
+                                end;
         }.
 
   End MODSIM.
